\begin{tikzpicture}[->]
    \node[latent] (zm) {$\myz[t-1]$};
    \node[latent,right=of zm, xshift=-3mm] (z) {$\myz[t]$};
    \node[latent,right=of z, xshift=-3mm] (zp) {$\myz[t+1]$};
    \node[obs,below=of zm, yshift=1mm] (xm) {$\myx[t-1]$};
    \node[obs,right=of xm, xshift=-3mm] (x) {$\myx[t]$};
    \node[obs,right=of x, xshift=-3mm] (xp) {$\myx[t+1]$};
    \node[latent,left=of zm,yshift=-9mm, xshift=5mm] (v) {$\myv$};
    \edge {zm} {xm,z};
    \edge{z} {x,zp};
    \edge{zp} {xp};
    \path (zm) edge[bend left] (zp);
    \path (v) edge[bend left] (xm);
    \path (v) edge[bend left] (x);
    \path (v) edge[bend left] (xp);
\end{tikzpicture}
