\begin{tikzpicture}[->]
    \node[latent] (zm) {$\myz[t-1]$};
    \node[latent,right=of zm] (z) {$\myz[t]$};
    \node[latent,right=of z] (zp) {$\myz[t+1]$};
    \node[obs,below=of zm] (xm) {$\myx[t-1]$};
    \node[obs,right=of xm] (x) {$\myx[t]$};
    \node[obs,right=of x] (xp) {$\myx[t+1]$};
    \edge{zm} {z};
    \edge{z} {zp};
    %\path(zm) edge[bend left=30] (zp);
    \edge{xm} {zm};
    \edge[blue]{xm} {z};
    \edge[blue]{xm} {zp};
    \edge{x} {zm};
    \edge{x} {z};
    \edge[blue]{x} {zp};
    \edge{xp} {zm};
    \edge{xp} {z};
    \edge{xp} {zp};
\end{tikzpicture}
