\begin{tikzpicture}[->]
    \node[latent] (zm) {$\myz[t-1]$};
    \node[latent,right=of zm] (z) {$\myz[t]$};
    \node[latent,right=of z] (zp) {$\myz[t+1]$};
    \node[obs,below=of zm] (xm) {$\myx[t-1]$};
    \node[obs,right=of xm] (x) {$\myx[t]$};
    \node[obs,right=of x] (xp) {$\myx[t+1]$};
    \edge {zm} {xm,x,xp,z};
    \edge{z} {x,xp,zp};
    \edge{x,zp} {xp};
    \edge{x} {zp};
    \edge{xm} {x,z,zp};
    \path (xm) edge[bend right] (xp);
    \path (zm) edge[bend left] (zp);
\end{tikzpicture}
