\begin{tikzpicture}[->]
    \node[latent] (zm) {$\myz[t-1]$};
    \node[latent,right=of zm] (z) {$\myz[t]$};
    \node[latent,right=of z] (zp) {$\myz[t+1]$};
    \node[det,below=of zm, yshift=3mm] (hm) {$\myh[t-1]$};
    \node[det,right=of hm,xshift=-2mm] (h) {$\myh[t]$};
    \node[det,right=of h,xshift=-2.5mm] (hp) {$\myh[t+1]$};
    \node[obs,below=of hm, yshift=3mm] (xm) {$\myx[t-1]$};
    \node[obs,right=of xm] (x) {$\myx[t]$};
    \node[obs,right=of x] (xp) {$\myx[t+1]$};
    \edge {hm} {zm};
    \edge {hm} {xm};
    \edge{hm,zm,xm} {h};
    \edge{h} {x,z};
    \edge{h,x,z} {hp};
    \edge{hp} {zp,xp};
    \path (zm) edge[bend left] (xm);
    \path (z) edge[bend left] (x);
    \path (zp) edge[bend left] (xp);
\end{tikzpicture}
